Add `(a : α)` to `ReadWrite.sleep` and show it still works. We probably don't actually need this for `sleep` specifically since there's no state that comes after

ReadWrite.lean
@@ -5,17 +5,17 @@
 -- `ReadWrite δ α`
 -- `δ`: type of data, like `Integer` or `SimpleIOData`
 inductive ReadWrite (δ : Type) : Type v → Type _
-| pure (a : α)                      : ReadWrite δ α
-| write (d : δ) (a : α)             : ReadWrite δ α
-| sleep (n : Nat) (h : n ≠ 0)       : ReadWrite δ α
-| read (next : ReadWrite δ (δ → α)) : ReadWrite δ α
+| pure (a : α)                        : ReadWrite δ α
+| write (d : δ) (a : α)               : ReadWrite δ α
+| sleep (n : Nat) (h : n ≠ 0) (a : α) : ReadWrite δ α -- we probably don't
+| read (next : ReadWrite δ (δ → α))   : ReadWrite δ α
 
 namespace ReadWrite
 
 def map (f : α → β) : ReadWrite δ α → ReadWrite δ β
   | .pure a => .pure (f a)
   | .write d a => .write d (f a)
-  | .sleep n h => .sleep n h
+  | .sleep n h a => .sleep n h (f a)
   | .read next => .read <| map (f ∘ ·) next
 
 @[simp]
@@ -30,15 +30,21 @@ def _root_.Function.swap (f : α → β → γ) : β → α → γ :=
 def tryDeepWrite (toWrite : δ) : ReadWrite δ α → ReadWrite δ α
   | .pure a => .write toWrite a
   | .write written a => .write written a
-  | .sleep n h => .sleep n h
+  | .sleep n h a => .sleep n h a
   | .read next => .read (tryDeepWrite toWrite next)
+
+def tryDeepSleep (n : Nat) (h : n ≠ 0) : ReadWrite δ α → ReadWrite δ α
+  | .pure a => .sleep n h a
+  | .write written a => .write written a
+  | .sleep n h a => .sleep n h a -- We can't add the `n`s or anything without losing the lawful property
+  | .read next => .read (tryDeepSleep n h next)
 
 -- Get `f ← mf`, then apply it to `a ← (ma ())`. If `f` and `x` both write, keep the write from `f`.
 def seq (mf : ReadWrite δ (α → β)) (ma : Unit → ReadWrite δ α) : ReadWrite δ β :=
   match mf with
   | .pure f => map f (ma ())
   | .write d f => tryDeepWrite d (map f (ma ()))
-  | .sleep n h => .sleep n h
+  | .sleep n h f => tryDeepSleep n h (map f (ma ()))
   | .read nextF => .read (seq (map Function.swap nextF) ma)
 termination_by sizeOf mf
 
@@ -52,6 +58,12 @@ theorem map_writeIfNotAlreadyWritten {d : δ} {f : α → β} {x : ReadWrite δ 
   cases x <;> try rfl
   simp only [tryDeepWrite, map, read.injEq]
   apply map_writeIfNotAlreadyWritten
+
+theorem map_tryDeepSleep {f : α → β} {x : ReadWrite δ α}
+    : map f (tryDeepSleep n h x) = tryDeepSleep n h (map f x) := by
+  cases x <;> try rfl
+  simp only [tryDeepSleep, map, read.injEq]
+  apply map_tryDeepSleep
 
 /-- The fundamental property of `writeIfNotAlreadyWritten`. -/
 theorem writeIfNotAlreadyWritten_idempotent {x : ReadWrite δ α}
@@ -86,28 +98,49 @@ theorem seq_pure {α β} (g : ReadWrite δ (α → β)) (a : α)
   cases g
   · simp [seq, map]
   · simp [seq, map, tryDeepWrite]
-  · simp only [seq, map]
+  · simp only [seq, map, tryDeepSleep]
   · rename_i next
     simp only [seq, map]
     congr 1
     rw [seq_pure, ←comp_map]
     rfl
 
+theorem tryDeepWrite_tryDeepSleep_idempotent : tryDeepWrite d (tryDeepSleep n h x) = tryDeepSleep n h x := by
+  induction x <;> simp only [tryDeepWrite, tryDeepSleep]
+  congr
+
+theorem tryDeepSleep_tryDeepWrite_idempotent : tryDeepSleep n h (tryDeepWrite d x) = tryDeepWrite d x := by
+  induction x <;> simp only [tryDeepSleep, tryDeepWrite]
+  congr
+
+theorem tryDeepSleep_idempotent : tryDeepSleep n' h' x = tryDeepSleep n h (tryDeepSleep n' h' x) := by
+  induction x <;> simp only [tryDeepSleep]
+  congr
+
 theorem seq_writeIfNotAlreadyWritten {α β} {d : δ} {g : ReadWrite δ (α → β)} {x : ReadWrite δ α}
     : seq (tryDeepWrite d g) (fun _ => x) = tryDeepWrite d (seq g fun _ => x) := by
   cases g
   · simp [tryDeepWrite, seq]
   · simp [tryDeepWrite, seq, writeIfNotAlreadyWritten_idempotent]
-  · simp [tryDeepWrite, seq]
+  · simp [tryDeepWrite, seq, ←map_tryDeepSleep, ←map_writeIfNotAlreadyWritten, tryDeepWrite_tryDeepSleep_idempotent]
   · simp only [tryDeepWrite, seq]
     rw [map_writeIfNotAlreadyWritten, seq_writeIfNotAlreadyWritten]
+
+theorem seq_tryDeepSleep {α β} {g : ReadWrite δ (α → β)} {x : ReadWrite δ α}
+    : seq (tryDeepSleep n h g) (fun _ => x) = tryDeepSleep n h (seq g fun _ => x) := by
+  cases g
+  · simp [tryDeepSleep, seq]
+  · simp [tryDeepSleep, seq, tryDeepSleep_tryDeepWrite_idempotent]
+  · simp [tryDeepSleep, seq, ←tryDeepSleep_idempotent]
+  · simp only [tryDeepSleep, seq]
+    rw [map_tryDeepSleep, seq_tryDeepSleep]
 
 theorem map_seq_r {α β γ} {f : β → γ} {g : ReadWrite δ (α → β)} {a : ReadWrite δ α}
     : map f (seq g fun _ => a) = seq (map (f ∘ ·) g) fun _ => a := by
   cases g
   · simp [pure_seq, map_pure, comp_map]
   · simp [seq, map_writeIfNotAlreadyWritten, map, comp_map]
-  · simp [seq, map]
+  · simp [seq, map, map_tryDeepSleep, comp_map]
   · simp only [map, seq]
     congr 1
     rw [map_seq_r, ←comp_map, ←comp_map]
@@ -118,6 +151,7 @@ theorem seq_assoc {α β γ} (a : ReadWrite δ α) (g : ReadWrite δ (α → β)
   cases h <;> simp only [seq, map]
   · simp [map_seq_r]
   · rw [seq_writeIfNotAlreadyWritten, map_seq_r]
+  · rw [map_seq_r, seq_tryDeepSleep]
   · rw [map_seq_r, ←comp_map, seq_assoc]
     simp only [←comp_map]
     rfl
